\documentclass[12pt]{article}
\usepackage[top=1in, bottom=1in, left=1in, right=1in]{geometry}
\usepackage{mathtools}
\usepackage{amsmath}
\usepackage{amsfonts}
\usepackage{amssymb}
\begin{document}
\title{Causal Set Research Notes}
\author{Will Cunningham}
\maketitle

\section{Patch Volume}
\subsection{1+1 Dimensions}

\begin{equation}
\begin{split}
\mathrm{d}V &= (a\mathrm{sec}\eta)^{\mathrm{d}+1} \, \mathrm{d}\eta \, \mathrm{d}\Phi_d \\
   &= a^2\mathrm{sec}^2\eta \, \mathrm{d}\eta \, \mathrm{d}\theta
\end{split}
\end{equation}

\begin{equation}
\begin{split}
V &= a^2\int_0^{\eta_0} \! \mathrm{d}\eta \int_0^{2\pi} \! \mathrm{d}\theta \, \mathrm{sec}^2\eta \\
  &= 2\pi a^2 \int_0^{\eta_0} \! \mathrm{sec}^2\eta \, \mathrm{d}\eta \\
  &= 2\pi a^2\mathrm{tan}\eta_0
\end{split}
\end{equation}

\begin{equation}
\begin{split}
N &= \delta V \\
\therefore N_{\mathrm{1+1}} &= 2\pi\delta a^2 \mathrm{tan}\eta_0
\end{split}
\end{equation}

\subsection{3+1 Dimensions}

\begin{equation}
\mathrm{d}V = a^4 \mathrm{sec}^4\eta \, \mathrm{d}\eta \, \mathrm{sin}^2\phi \, \mathrm{sin}\chi \, \mathrm{d}\phi \, \mathrm{d}\chi \, \mathrm{d}\theta
\end{equation}

\begin{equation}
\begin{split}
V &= a^4 \int_0^{\eta_0} \! \mathrm{d}\eta \int_0^{2\pi} \! \mathrm{d}\theta \int_0^\pi \! \mathrm{d}\chi \int_0^\pi \! \mathrm{d}\phi \, \mathrm{sec}^4\eta \, \mathrm{sin}^2\phi \, \mathrm{sin}\chi \\
  &= 2\pi a^4 \int_0^{\eta_0} \! \mathrm{d}\eta \int_0^\pi \! \mathrm{d}\chi \int_0^\pi \! \mathrm{d}\phi \, \mathrm{sec}^4\eta \, \mathrm{sin}^2\phi \, \mathrm{sin}\chi \\
  &= 4\pi a^4 \int_0^{\eta_0} \! \mathrm{d}\eta \int_0^\pi \! \mathrm{d}\phi \, \mathrm{sec}^4\eta \, \mathrm{sin}^2\phi \\
  &= 2\pi^2 a^4 \int_0^{\eta_0} \! \mathrm{sec}^4\eta \, \mathrm{d}\eta \\
  &= \frac{2}{3}\pi^2 a^4 \, (2+\mathrm{sec}^2\eta_0) \, \mathrm{tan}\eta_0
\end{split}
\end{equation}

\begin{equation}
\begin{split}
N &= \delta V \\
\therefore N_{\mathrm{3+1}} &= \frac{2}{3}\pi^2\delta a^4 \, (2+\mathrm{sec}^2\eta_0) \, \mathrm{tan}\eta_0
\end{split}
\end{equation}

\section{Expected Average Degrees}
\subsection{1+1 Dimensions}

\begin{equation}
\rho = \frac{\mathrm{sec}^2\eta}{\mathrm{tan}\eta_0}
\end{equation}

\begin{equation}
V_p = \mathrm{ln} \, \mathrm{sec}\eta
\end{equation}

\begin{equation}
\begin{split}
\langle V_p \rangle &= \int_0^{\eta_0} \! \frac{\mathrm{sec}^2\eta}{\mathrm{tan}\eta_0} \, \mathrm{ln} \, \mathrm{sec}\eta \, \mathrm{d}\eta \\
  &= \frac{1}{\mathrm{tan}\eta_0} \, \lbrack \eta + \mathrm{tan}\eta (\mathrm{ln} \, \mathrm{sec}\eta - 1) \rbrack_0^{\eta_0} \\
  &= \frac{1}{\mathrm{tan}\eta_0} \, \lbrack \eta_0 + \mathrm{tan}\eta_0 (\mathrm{ln} \, \mathrm{sec}\eta_0 - 1) \rbrack \\
  &= \frac{\eta_0}{\mathrm{tan}\eta_0} + \mathrm{ln} \, \mathrm{sec}\eta_0 - 1
\end{split}
\end{equation}

\begin{equation}
V_f = (\eta_0 - \eta) \, \mathrm{tan}\eta_0 + \mathrm{ln} \, \left(\frac{\mathrm{sec}\eta}{\mathrm{sec}\eta_0}\right)
\end{equation}

\begin{equation}
\begin{split}
\langle V_f \rangle &= \int_0^{\eta_0} \! \frac{\mathrm{sec}^2\eta}{\mathrm{tan}\eta_0} \left[ (\eta_0 - \eta) \, \mathrm{tan}\eta_0 + \ln\left(\frac{\sec\eta}{\sec\eta_0}\right) \right] \, \mathrm{d}\eta \\
  &= \frac{1}{\tan\eta_0} \left[ \eta_0\tan\eta_0 \int_0^{\eta_0} \! \sec^2\eta \, \mathrm{d}\eta - \tan\eta_0 \int_0^{\eta_0} \! \eta\sec^2\eta \, \mathrm{d}\eta \right. \\ & \left.\,\,\,\,\, + \int_0^{\eta_0} \! \sec^2\eta\ln\sec\eta \, \mathrm{d}\eta - \ln\sec\eta_0 \int_0^{\eta_0} \! \sec^2\eta \, \mathrm{d}\eta \right] \\
  &= \frac{1}{\tan\eta_0} \left[ \eta_0\tan^2\eta_0 - \eta_0\tan^2\eta_0 + \tan\eta_0\ln\sec\eta_0 \right. \\ & \left. \,\,\,\,\, + \eta_0 + \tan\eta_0\left(\ln\sec\eta_0 - 1\right) - \tan\eta_0\ln\sec\eta_0 \right] \\
  &= \frac{\eta_0}{\tan\eta_0} + \ln\sec\eta_0 - 1
\end{split}
\end{equation}

\begin{equation}
\begin{split}
\therefore \langle V_p \rangle &= \langle V_f \rangle \\
\therefore \langle \bar{k} \rangle &= 2a^2\delta \left( \langle V_p \rangle + \langle V_f \rangle \right) \\
  &= 4 \delta a^2 \left( \frac{\eta_0}{\tan\eta_0} + \ln\sec\eta_0 - 1 \right)
\end{split}
\end{equation}

\subsection{3+1 Dimensions}

\begin{equation}
\rho = \frac{3\sec^4\eta}{\left( 2 + \sec^2\eta_0 \right) \tan\eta_0}
\end{equation}

\begin{equation}
\begin{split}
V_p(\eta) &= \int_0^\eta \! \mathrm d \eta^\prime \int_0^{\eta - \eta^\prime} \! 2\mathrm d \theta \int_0^\pi \! \mathrm d \phi \int_0^\pi \! \mathrm d \chi \, a^4\sec^4\eta^\prime \, \sin^2\phi \, \sin\chi \\
  & \;\;\;\;\;\;\;\;\;\; \int_0^\pi \! \sin\chi \, \mathrm d \chi = 2 \\
  & \;\;\;\;\;\;\;\;\;\; \int_0^\pi \! \sin^2\phi \, \mathrm d \phi = \frac{\pi}{2} \\
  & \;\;\;\;\;\;\;\;\;\; \int_0^{\eta - \eta^\prime} \! 2\,\mathrm d\theta = 2\left(\eta - \eta^\prime\right) \\
  &= 2\pi a^4 \int_0^\eta \! \left(\eta - \eta^\prime\right)\sec^4\eta^\prime\,\mathrm d\eta^\prime \\
  & \;\;\;\;\;\;\;\;\;\; \int_0^\eta \! \sec^4\eta^\prime \, \mathrm d\eta^\prime = \frac{1}{3}\tan\eta\left(2+\sec^2\eta\right) \\
  & \;\;\;\;\;\;\;\;\;\; \int_0^\eta \! \eta^\prime\sec^4\eta^\prime\,\mathrm d\eta^\prime = \frac{1}{3}\left(-2\ln\sec\eta - \frac{1}{2}\sec^2\eta + 2\eta\tan\eta + \eta\sec^2\eta\tan\eta + \frac{1}{2}\right) \\
  &= 2\pi a^4\left(\frac{2}{3}\eta\tan\eta + \frac{1}{3}\eta\sec^2\eta + \frac{2}{3}\ln\sec\eta + \frac{1}{6}\sec^2\eta - \frac{2}{3}\eta\tan\eta - \frac{1}{3}\eta\sec^2\eta\tan\eta - \frac{1}{6}\right) \\
  &= 2\pi a^4\left(\frac{1}{3}\eta\sec^2\eta + \frac{2}{3}\ln\sec\eta + \frac{1}{6}\sec^2\eta - \frac{1}{3}\eta\sec^2\eta\tan\eta - \frac{1}{6}\right) \\
  &= \frac{2}{3}\pi a^4 \left(\eta\sec^2\eta + 2\ln\sec\eta + \frac{1}{2}\sec^2\eta - \eta\sec^2\eta\tan\eta - \frac{1}{2}\right)
\end{split}
\end{equation}

\begin{equation}
\begin{split}
\langle\bar{k_o}\rangle &= \int_0^{\eta0} \! \rho\delta V_p(\eta)\,\mathrm d\eta \\
  &= \frac{2\pi\delta a^4}{(2+\sec^2\eta_0)\tan\eta_0} \int_0^{\eta_0} \left(\eta\sec^6\eta + \sec^4\ln\sec^2\eta + \frac{1}{2}\sec^6\eta \right. \\ \,\,\,\,\, \left. - \eta\sec^6\eta\tan\eta - \frac{1}{2}\sec^4\eta\right)\,\mathrm d\eta \\
  & \;\;\;\;\;\;\;\;\;\; \int_0^{\eta_0}\! \eta\sec^6\eta\,\mathrm d\eta = -\frac{8}{15}\ln\sec\eta_0 - \frac{2}{15}\sec^2\eta_0 - \frac{1}{20}\sec^4\eta_0 + \frac{8}{15}\eta_0\tan\eta_0 \\ \;\;\;\;\;\;\;\;\;\;\,\,\,\,\, + \frac{4}{15}\eta_0\sec^2\eta_0\tan\eta_0 + \frac{1}{5}\eta_0\sec^4\eta_0\tan\eta_0 + \frac{11}{60} \\
  & \;\;\;\;\;\;\;\;\;\; \int_0^{\eta_0} \! \sec^4\eta\ln\sec\eta\,\mathrm d\eta = \frac{2}{3}\eta_0 - \frac{5}{9}\tan\eta_0 - \frac{1}{9}\sec^2\eta_0\tan\eta_0 \\ \;\;\;\;\;\;\;\;\;\;\,\,\,\,\, + \frac{1}{3}\ln\sec\eta_0\sec^2\eta_0\tan\eta_0 + \frac{2}{3}\ln\sec\eta_0\tan\eta_0 \\
  & \;\;\;\;\;\;\;\;\;\; \int_0^{\eta_0} \! \sec^6\eta\,\mathrm d\eta = \frac{8}{15}\tan\eta_0 + \frac{4}{15}\sec^2\eta_0\tan\eta_0 + \frac{1}{5}\sec^4\eta_0\tan\eta_0 \\
  & \;\;\;\;\;\;\;\;\;\; \int_0^{\eta_0} \! \eta\sec^6\eta\tan\eta\,\mathrm d\eta = \frac{1}{6}\eta_0\sec^6\eta_0 - \frac{4}{45}\tan\eta_0 - \frac{2}{45}\sec^2\eta_0\tan\eta_0 - \frac{1}{30}\sec^4\eta_0\tan\eta_0 \\
  & \;\;\;\;\;\;\;\;\;\; \int_0^{\eta_0} \! \sec^4\eta\,\mathrm d\eta = \frac{2}{3}\tan\eta_0 + \frac{1}{3}\sec^2\eta_0\tan\eta_0 \\


\end{document}
